src/Distributions/BernoulliExpNeg/Equivalence.dfy
@@ -34,7 +34,7 @@ module BernoulliExpNeg.Equivalence {
     calc {
       Model.GammaLe1Loop(gamma)(ak)(s);
       { reveal Model.GammaLe1Loop(); }
-      Loops.While(Model.GammaLe1LoopCondition, Model.GammaLe1LoopIter(gamma), ak)(s);
+      Loops.While(Model.GammaLe1LoopCondition, Model.GammaLe1LoopIter(gamma))(ak)(s);
       { reveal Model.GammaLe1Loop();
         Loops.WhileUnroll(Model.GammaLe1LoopCondition, Model.GammaLe1LoopIter(gamma), ak, s); }
       Monad.Bind(Model.GammaLe1LoopIter(gamma)(ak), Model.GammaLe1Loop(gamma))(s);
